examples/hoare_logic/blocking_semantics3/blocking_semantics3_ImpExpr_eval_swap_any_1.v
@@ -441,54 +441,29 @@ Axiom eval_swap_term : forall (t:term) (sigma:(map mident value)) (pi:(list
   (~ (id1 = id2)) -> ((eval_term sigma (Cons (id1, v1) (Cons (id2, v2) pi))
   t) = (eval_term sigma (Cons (id2, v2) (Cons (id1, v1) pi)) t)).
 
-Axiom eval_swap_any : forall (f:fmla) (sigma:(map mident value)) (pi:(list
-  (ident* value)%type)) (l:(list (ident* value)%type)) (id1:ident)
-  (id2:ident) (v1:value) (v2:value), (~ (id1 = id2)) -> ((eval_fmla sigma
-  (infix_plpl l (Cons (id1, v1) (Cons (id2, v2) pi))) f) <-> (eval_fmla sigma
-  (infix_plpl l (Cons (id2, v2) (Cons (id1, v1) pi))) f)).
-
 (* Why3 goal *)
-Theorem eval_swap : forall (f:fmla),
+Theorem eval_swap_any : forall (f:fmla),
   match f with
   | (Fterm t) => True
   | (Fand f1 f2) => True
   | (Fnot f1) => True
   | (Fimplies f1 f2) => True
   | (Flet i t f1) => (forall (sigma:(map mident value)) (pi:(list (ident*
-      value)%type)) (id1:ident) (id2:ident) (v1:value) (v2:value),
-      (~ (id1 = id2)) -> ((eval_fmla sigma (Cons (id1, v1) (Cons (id2, v2)
-      pi)) f1) <-> (eval_fmla sigma (Cons (id2, v2) (Cons (id1, v1) pi))
+      value)%type)) (l:(list (ident* value)%type)) (id1:ident) (id2:ident)
+      (v1:value) (v2:value), (~ (id1 = id2)) -> ((eval_fmla sigma
+      (infix_plpl l (Cons (id1, v1) (Cons (id2, v2) pi))) f1) <->
+      (eval_fmla sigma (infix_plpl l (Cons (id2, v2) (Cons (id1, v1) pi)))
       f1))) -> forall (sigma:(map mident value)) (pi:(list (ident*
-      value)%type)) (id1:ident) (id2:ident) (v1:value) (v2:value),
-      (~ (id1 = id2)) -> ((eval_fmla sigma (Cons (id1, v1) (Cons (id2, v2)
-      pi)) f) -> (eval_fmla sigma (Cons (id2, v2) (Cons (id1, v1) pi)) f))
+      value)%type)) (l:(list (ident* value)%type)) (id1:ident) (id2:ident)
+      (v1:value) (v2:value), (~ (id1 = id2)) -> ((eval_fmla sigma
+      (infix_plpl l (Cons (id1, v1) (Cons (id2, v2) pi))) f) ->
+      (eval_fmla sigma (infix_plpl l (Cons (id2, v2) (Cons (id1, v1) pi)))
+      f))
   | (Fforall i d f1) => True
   end.
 destruct f; auto.
-intros H sigma pi id1 id2 v1 v2 H1 H2.
+intros.
 simpl in *.
-rewrite eval_swap_term in H2; auto.
-destruct (ident_decide i id2).
-(* i = id1*)
-subst.
-apply H in H2; auto.
-destruct (ident_decide i id1).
-(* i = id1*)
-subst.
-apply H; auto.
-
-
-
-simpl in *.
-rewrite eval_swap_term in H2; auto.
-apply eval_same_var.
-
-
-
-
- eval_same_var_term.
-
-(* i <> id2*)
 
 Qed.
 
